# Ejercicios
$$
f(x) = \frac{2x^2 - x}{2x^3 + 7x}
$$
$$
f'(x) = \frac{(2x^3 + 7x )\frac{d}{dx} (2x^2 - x) - (2x^2 - x)\frac{d}{dx} (2x^3 + 7x )}{(2x^3 + 7x)^2}
$$
$$
f'(x) = \frac{(2x^3 + 7x )(4x - 1) - (2x^2 - x)(6x^2 + 7 )}{(2x^3 + 7x)^2}
$$
$$
f'(x) = \frac{(8x^4 - 2x^3  + 28x^2 - 7x) - (12x^4 - 6x^3 + 14x^2 - 7x )}{(2x^3 + 7x)^2}
$$
$$
f'(x) = \frac{(8x^4 - 2x^3  + 28x^2 - 7x) - (12x^4 - 6x^3 + 14x^2 - 7x )}{(2x^3 + 7x)^2}
$$
$$
rf_{3}
$$
$$
f'(x) = \frac{- 4x^4 + 4x^3  + 14x^2 }{(2x^3 + 7x)^2}
$$
